{
 "cells": [
  {
   "cell_type": "markdown",
   "metadata": {},
   "source": [
    "This one took me a few goes to get through propertly, so I thought it was worth recording it step-by-step here...\n",
    "\n",
    "**Calculate the derivative with respect to $x$ of the following:**\n",
    "\n",
    "$f(x)=\\arctan\\Big(\\frac{x}{\\sqrt{1-x^2}}\\Big)$\n",
    "\n",
    "To simplify things, let's just focus on the bit inside the brackets - call that $g(x)$...\n",
    "\n",
    "$g(x)=\\frac{x}{\\sqrt{1-x^2}}$\n",
    "\n",
    "...so...\n",
    "\n",
    "$f(x)=\\arctan(g(x))$\n",
    "\n",
    "Now, let's find $g'(x)$:\n",
    "\n",
    "$g(x)=\\frac{x}{\\sqrt{1-x^2}}$\n",
    "\n",
    "$=\\frac{x}{(1-x^2)^{\\frac{1}{2}}}$\n",
    "\n",
    "$=x(1-x^2)^{-\\frac{1}{2}}$\n",
    "\n",
    "...which we can differentiate with a combination of the chain rule & product rule...\n",
    "\n",
    "$g'(x)=1.(1-x^2)^{-\\frac{1}{2}}+x.(-\\frac{1}{2}(1-x^2)^{-\\frac{3}{2}}.(-2x))$\n",
    "\n",
    "$=(1-x^2)^{-\\frac{1}{2}}+x^2(1-x^2)^{-\\frac{3}{2}}$\n",
    "\n",
    "$=\\frac{1}{(1-x^2)^{\\frac{1}{2}}}+\\frac{x^2}{(1-x^2)^{\\frac{3}{2}}}$\n",
    "\n",
    "$=\\frac{(1-x^2)+x^2}{(1-x^2)^{\\frac{3}{2}}}$\n",
    "\n",
    "$g'(x)=\\frac{1}{(1-x^2)^{\\frac{3}{2}}}$\n",
    "\n",
    "Now, treat it like an \"Implicit differentiation & inverse function\" problem:\n",
    "\n",
    "$f(x)=\\arctan(g(x))$\n",
    "\n",
    "$\\tan(f(x))=g(x)$\n",
    "\n",
    "Differentiating both sides...\n",
    "\n",
    "$\\sec^2(f(x))f'(x)=g'(x)$\n",
    "\n",
    "$\\sec^2(f(x))f'(x)=\\frac{1}{(1-x^2)^{\\frac{3}{2}}}$\n",
    "\n",
    "$f'(x)=\\frac{1}{(1-x^2)^{\\frac{3}{2}}\\sec^2(f(x))}$\n",
    "\n",
    "$=\\frac{1}{(1-x^2)^{\\frac{3}{2}}\\sec^2\\big(\\arctan(\\frac{x}{\\sqrt{1-x^2}})\\big)}$\n",
    "\n",
    "...which is a very complicated version of the correct answer! Let's simplify it with some trigonometry...\n",
    "\n",
    "Our initial function, $f(x)=\\arctan\\Big(\\frac{x}{\\sqrt{1-x^2}}\\Big)$, can be interpreted as \"the angle, say $\\theta$, such that $\\tan\\theta=\\frac{x}{\\sqrt{1-x^2}}$, and if we look at [$\\tan$ and $\\sec$ in the context of the unit circle](0c.%20Trigonometric%20functions%20and%20the%20unit%20circle.ipynb#tan-and-sec), we can calculate $\\sec^2$ of this angle using pythagoras...\n",
    "\n",
    "![](img\\sec-pythagoras.jpg)\n",
    "\n",
    "$\\sec^2=\\Big(\\frac{x}{\\sqrt{1-x^2}}\\Big)^2+1^2$\n",
    "\n",
    "$=\\frac{x^2}{1-x^2}+1$\n",
    "\n",
    "$=\\frac{x^2}{1-x^2}+\\frac{1-x^2}{1-x^2}$\n",
    "\n",
    "$=\\frac{x^2+1-x^2}{1-x^2}$\n",
    "\n",
    "$=\\frac{1}{1-x^2}$\n",
    "\n",
    "So, plugging that in to our derivative...\n",
    "\n",
    "$f'(x)=\\frac{1}{(1-x^2)^{\\frac{3}{2}}\\sec^2(f(x))}$\n",
    "\n",
    "$=\\frac{1}{(1-x^2)^{\\frac{3}{2}}\\frac{1}{1-x^2}}$\n",
    "\n",
    "$=\\frac{1-x^2}{(1-x^2)^{\\frac{3}{2}}}$\n",
    "\n",
    "That denominator, $(1-x^2)^{\\frac{3}{2}}$, can be written as $(1-x^2)(1-x^2)^{\\frac{1}{2}}$, using the [rules of exponents](0.%20References.ipynb#Exponents-refresher) ($a^1=a$ and $a^xa^y=a^{x+y}$), so...\n",
    "\n",
    "$f'(x)=\\frac{1-x^2}{(1-x^2)(1-x^2)^{\\frac{1}{2}}}$\n",
    "\n",
    "$=\\frac{1}{(1-x^2)^{\\frac{1}{2}}}$\n",
    "\n",
    "$=\\frac{1}{\\sqrt{1-x^2}}$\n",
    "\n",
    "...which is a much, much nicer version of the answer!"
   ]
  }
 ],
 "metadata": {
  "kernelspec": {
   "display_name": "Octave",
   "language": "octave",
   "name": "octave"
  },
  "language_info": {
   "file_extension": ".m",
   "help_links": [
    {
     "text": "GNU Octave",
     "url": "https://www.gnu.org/software/octave/support.html"
    },
    {
     "text": "Octave Kernel",
     "url": "https://github.com/Calysto/octave_kernel"
    },
    {
     "text": "MetaKernel Magics",
     "url": "https://github.com/calysto/metakernel/blob/master/metakernel/magics/README.md"
    }
   ],
   "mimetype": "text/x-octave",
   "name": "octave",
   "version": "4.2.1"
  }
 },
 "nbformat": 4,
 "nbformat_minor": 2
}
